code/ecdsap256/Hacl.Impl.P256.LowLevel.PrimeSpecific.fsti
@@ -27,8 +27,10 @@ p384_prime_list) /\ recallable x /\ felem_seq_as_nat P384 (Lib.Sequence.of_list 
 
 
 inline_for_extraction
-let prime_buffer (#c: curve) (x: glbuffer uint64 (getCoordinateLenU64 c) {witnessed #uint64 #(getCoordinateLenU64 c) x (Lib.Sequence.of_list (prime_list c)) /\ recallable x /\ felem_seq_as_nat c (Lib.Sequence.of_list (prime_list c)) == getPrime c}) = 
-  createL_global (prime_list c)
+let prime_buffer (#c: curve): (x: glbuffer uint64 (getCoordinateLenU64 c) {witnessed #uint64 #(getCoordinateLenU64 c) x (Lib.Sequence.of_list (prime_list c)) /\ recallable x /\ felem_seq_as_nat c (Lib.Sequence.of_list (prime_list c)) == getPrime c}) = 
+  match c with
+  | P256 -> prime256_buffer
+  | P384 -> prime384_buffer
 
 
 val reduction_prime_2prime_with_carry: #c: curve -> x: widefelem c -> result: felem c -> 
