code/ecdsap256/Hacl.Impl.P384.LowLevel.fst
@@ -1,0 +1,31 @@
+module Hacl.Impl.P384.LowLevel
+
+open FStar.HyperStack.All
+open FStar.HyperStack
+module ST = FStar.HyperStack.ST
+
+open Lib.IntTypes
+open Lib.Buffer
+
+open Hacl.Spec.P256.Definition
+open Hacl.Lemmas.P256
+(* open Spec.ECDSA.Lemmas *)
+open Spec.P256
+open Spec.ECDSA
+
+open FStar.Math
+open FStar.Math.Lemmas
+open FStar.Mul
+
+open FStar.Tactics
+open FStar.Tactics.Canon 
+
+(* open Spec.P256.Lemmas *)
+open Lib.IntTypes.Intrinsics
+
+
+val square_p384: f: felem P384 -> out: widefelem P384 -> Stack unit
+    (requires fun h -> live h out /\ live h f /\ eq_or_disjoint f out)
+    (ensures  fun h0 _ h1 -> modifies (loc out) h0 h1 /\ wide_as_nat P384 h1 out = as_nat P384 h0 f * as_nat P384 h0 f)
+
+let square_p384 f out = admit()
