code/ecdsap256/Hacl.Spec.P256.Definition.fst
@@ -46,7 +46,7 @@ let p384_prime_list : x:list uint64{List.Tot.length x == 6 /\
   let open FStar.Mul in 
   [@inline_let]
   let x =
-    [ (u64 0xffffffffffffffff);  (u64 0xffffffff); (u64 0);  (u64 0xffffffff00000001);] in
+    [ (u64 0xffffffff);  (u64 0xffffffff00000000); (u64 0xfffffffffffffffe);  (u64 0xffffffffffffffff); (u64 0xffffffffffffffff); (u64 0xffffffffffffffff);] in
     assert_norm(0xffffffff + 0xffffffff00000000 * pow2 64 + 0xfffffffffffffffe * pow2 128 + 
     0xffffffffffffffff * pow2 192 +  0xffffffffffffffff * pow2 256 +  0xffffffffffffffff * pow2 320 == prime384);
   x
